high-level-jasmin/maps/map_optimized_proof.ec
@@ -1,30 +1,33 @@
 require import AllCore IntDiv CoreMap List Distr.
 from Jasmin require import JModel_x86.
-require import Map_simple Loop Array16.
+require import Map_optimized Loop Array16.
 
 clone import LOOP as L with 
   type elem <- W64.t,
   op N <- 16,
   theory ArrayN <- Array16.
 
+clone import L.MAP_iter as I with
+  op iter <- 4.
+
 module Body = { 
   proc body = M.plus_one
 }.
 
-equiv map_simple_map : 
-  Map_simple.M.__map_simple_plus_one_u64_16 ~ 
-  L.MAP.Map(Body).map : ={arg} ==> ={res}.
-proof. by proc; inline *; sim. qed.
+equiv map_optimized_map : 
+  Map_optimized.M.__map_optimized_plus_one_u64_16_4 ~ 
+  I.Map(Body).map_incr : ={arg} ==> ={res}.
+proof. proc; inline *; sim. qed.
 
 op oplus_one (x : W64.t) = x + W64.of_int 1.
 
 hoare plus_one_spec x_ : M.plus_one : arg = x_ ==> res = oplus_one x_.
 proof. proc; auto => />. qed.
 
-hoare __map_simple_plus_one_u64_16_spec a_ : 
-  Map_simple.M.__map_simple_plus_one_u64_16 : 
+hoare __map_optimized_plus_one_u64_16_spec a_ : 
+  Map_optimized.M.__map_optimized_plus_one_u64_16_4 : 
     arg = a_ ==> 
     res = Array16.map oplus_one a_.
 proof.
-  conseq map_simple_map (MAP.map_spec Body oplus_one plus_one_spec a_) => // /#.
+  conseq map_optimized_map (I.map_incr_spec Body oplus_one plus_one_spec a_) => // /#.
 qed.
